integrated Util and Abstract_Rewriting extensions from IsaFoR

thys/Abstract-Rewriting/Abstract_Rewriting.thy
@@ -26,7 +26,7 @@ with IsaFoR/CeTA. If not, see <http://www.gnu.org/licenses/>.
 header {* Abstract Rewrite Systems *}
 
 theory Abstract_Rewriting
-imports Main Util
+imports Main Util "../Transitive-Closure/Transitive_Closure_Impl"
 begin
 
 lemma trancl_mono_set: "r \<subseteq> s \<Longrightarrow> r^+ \<subseteq> s^+"
@@ -228,6 +228,12 @@ proof -
     thus False by (induct) (auto simp: `\<forall>b. (a, b) \<notin> A`)
    qed
 qed
+
+lemma NF_Id_on_fst_image[simp]: "NF (Id_on (fst ` A)) = NF A" by force
+
+lemma fst_image_NF_Id_on[simp]: "fst ` R = Q \<Longrightarrow> NF (Id_on Q) = NF R" by force
+
+lemma NF_empty[simp]: "NF {} = UNIV" by auto
 
 lemma normalizability_I: "(a, b) \<in> A^* \<Longrightarrow> b \<in> NF A \<Longrightarrow> (a, b) \<in> A^!"
 by (simp add: normalizability_def)
@@ -530,6 +536,29 @@ lemma SN_imp_irreflexive: assumes "SN r" shows "(l,l) \<notin> r"
 proof
   assume in_gr: "(l,l) \<in> r"
   with `SN r` show False unfolding SN_defs by auto
+qed
+
+
+lemma SN_nat_bounded: "SN {(x,y :: nat). x < y \<and> y \<le> b}" (is "SN ?R")
+proof 
+  fix f
+  assume "\<forall> i. (f i, f (Suc i)) \<in> ?R"
+  hence steps: "\<And> i. (f i, f (Suc i)) \<in> ?R" ..
+  {
+    fix i
+    have inc: "f 0 + i \<le> f i"
+    proof (induct i)
+      case 0 thus ?case by auto
+    next
+      case (Suc i)
+      have "f 0 + Suc i \<le> f i + Suc 0" using Suc by simp
+      also have "... \<le> f (Suc i)" using steps[of i]
+        by auto
+      finally show ?case by simp
+    qed
+  }
+  from this[of "Suc b"] steps[of b]
+  show False by simp
 qed
 
 
@@ -1710,6 +1739,72 @@ proof (rule subsetI2)
   fix a b assume "(a,b) \<in> SN_rel R S" thus "(a,b) \<in> R" unfolding SN_rel_def by simp
 qed
 
+lemma first_step: assumes C: "C = A \<union> B" and steps: "(x,y) \<in> C^*"
+  and Bstep: "(y,z) \<in> B"
+  shows "\<exists> y. (x,y) \<in> A^* O B"
+  using steps
+proof (induct rule: converse_rtrancl_induct)
+  case base
+  show ?case using Bstep by auto
+next 
+  case (step u x)
+  from step(1)[unfolded C] 
+  show ?case
+  proof
+    assume "(u,x) \<in> B"
+    thus ?thesis by auto
+  next
+    assume ux: "(u,x) \<in> A"
+    from step(3) obtain y where "(x,y) \<in> A^* O B" by auto
+    then obtain z where "(x,z) \<in> A^*" and step: "(z,y) \<in> B" by auto
+    with ux have "(u,z) \<in> A^*" by auto
+    with step have "(u,y) \<in> A^* O B" by auto
+    thus ?thesis by auto
+  qed
+qed
+
+lemma first_step_O: assumes C: "C = A \<union> B" and steps: "(x,y) \<in> C^* O B"
+  shows "\<exists> y. (x,y) \<in> A^* O B"
+proof -
+  from steps obtain z where "(x,z) \<in> C^*" and "(z,y) \<in> B" by auto
+  from first_step[OF C this] show ?thesis .
+qed
+
+lemma firstStep: assumes LSR: "L = S \<union> R" and xyL: "(x,y) \<in> L^*"
+  shows "(x,y) \<in> R^* \<or> (x,y) \<in> R^* O S O L^*"
+proof (cases "(x,y) \<in> R^*")
+  case True
+  thus ?thesis by simp
+next
+  case False 
+  let ?SR = "S \<union> R"
+  from xyL and LSR have "(x,y) \<in> ?SR^*" by simp
+  from this and False have "(x,y) \<in> R^* O S O ?SR^*" 
+  proof (induct rule: rtrancl_induct)
+    case base thus ?case by simp
+  next
+    case (step y z)
+    thus ?case
+    proof (cases "(x,y) \<in> R^*")
+      case False with step have "(x,y) \<in> R^* O S O ?SR^*" by simp
+      from this obtain u where xu: "(x,u) \<in> R^* O S" and uy: "(u,y) \<in> ?SR^*" by force
+      from `(y,z) \<in> ?SR` have "(y,z) \<in> ?SR^*" by auto
+      with uy have "(u,z) \<in> ?SR^*" by (rule rtrancl_trans)
+      with xu show ?thesis by auto
+    next
+      case True 
+      have "(y,z) \<in> S" 
+      proof (rule ccontr)
+	assume "(y,z) \<notin> S" with `(y,z) \<in> ?SR` have "(y,z) \<in> R" by auto
+	with True  have "(x,z) \<in> R^*"  by auto
+	with `(x,z) \<notin> R^*` show False ..
+      qed
+      with True show ?thesis by auto
+    qed
+  qed
+  with LSR show ?thesis by simp
+qed  
+
 lemma union_iseq_SN_elt_imp_first_step:
   assumes "\<forall>i. (t i, t (Suc i)) \<in> (R \<union> S)" and "SN_elt S (t 0)"
   shows "\<exists>i. (t i, t (Suc i)) \<in> R \<and> (\<forall>j<i. (t j, t (Suc j)) \<in> S \<and> (t j, t (Suc j)) \<notin> R)"
@@ -1764,18 +1859,18 @@ qed
 
 lemmas SN_elt_mono = SN_elt_subset
 
+
+lemma rtrancl_fun_conv:
+  "((s,t) \<in> R^*) = (\<exists> f n. f 0 = s \<and> f n = t \<and> (\<forall> i < n. (f i, f (Suc i)) \<in> R))"
+  unfolding rtrancl_is_UN_rel_pow using rel_pow_fun_conv[where R = R]
+  by auto
+
+
 lemma rtrancl_imp_rel_pow': "(x,y) \<in> R^* \<Longrightarrow> \<exists>n. (x,y) \<in> ((R::'a ars) ^^ n)"
-proof (induct rule: rtrancl_induct)
-  case base thus ?case using rel_pow_0_I by best
-next
-  case (step y z)
-  then obtain n where "(x,y) \<in> (R ^^ n)" by best
-  with step have "(x,z) \<in> (R ^^ (Suc n))" using rel_pow_Suc_I by auto
-  thus ?case by best
-qed
+  unfolding rtrancl_is_UN_rel_pow by auto
 
 lemma compat_tr_compat: assumes "NS O S \<subseteq> S" shows "NS^* O S \<subseteq> S"
-using non_strict_into_strict[where S = S and NS = NS] assms by blast
+  using non_strict_into_strict[where S = S and NS = NS] assms by blast
 
 lemma right_comp_S[simp]:
   assumes "(x, y) \<in> S O (S O S^* O NS^* \<union> NS^*)"
@@ -1865,32 +1960,23 @@ qed
 
 lemma compatible_conv:
   assumes compat: "NS O S \<subseteq> S" 
-  shows "(NS \<union> S)^* O S O (NS \<union> S)^* = S O S^* O NS^*"
+  shows "(NS \<union> S)^* O S O (NS \<union> S)^* = S O S^* O NS^*" 
 proof -
   let ?NSuS = "NS \<union> S"
   let ?NSS = "S O S^* O NS^*"
   let ?midS = "?NSuS^* O S O ?NSuS^*"
-
-  have a: "NS^* \<subseteq> ?NSuS^*" using rtrancl_mono by blast
-  have "S^* \<subseteq> ?NSuS^*" using rtrancl_mono by blast
-  with a have b: "S^* O NS^* \<subseteq> ?NSuS^*" using rtrancl_trans[where r = ?NSuS] by blast
-  hence one: "?NSS \<subseteq> ?midS" using rtrancl_refl[where r = ?NSuS] by auto
-
+  have one: "?NSS \<subseteq> ?midS" by regexp 
   have "?NSuS^* O S \<subseteq> (?NSS \<union> NS^*) O S"
     using compatible_rtrancl_split[where S = S and NS = NS] compat by blast
   also have "\<dots> \<subseteq> ?NSS O S \<union> NS^* O S" by auto
   also have "\<dots> \<subseteq> ?NSS O S \<union> S" using compat compat_tr_compat[where S = S and NS = NS] by auto
-  also have "\<dots> \<subseteq> S O ?NSuS^* O S \<union> S" using b by auto
-  also have "\<dots> \<subseteq> S O ?NSuS^* O ?NSuS \<union> S" using rtrancl_mono[where r = S and s = ?NSuS] by auto
-  also have "\<dots> \<subseteq> S O ?NSuS^* \<union> S" using rtrancl_trans[where r = ?NSuS] rtrancl_refl[where r = ?NSuS] by blast
-  also have "\<dots> \<subseteq> S O ?NSuS^*" using rtrancl_refl[where r = ?NSuS] by auto
+  also have "\<dots> \<subseteq> S O ?NSuS^*" by regexp
   finally have "?midS \<subseteq> S O ?NSuS^* O ?NSuS^*" by blast
-  also have "\<dots> \<subseteq> S O ?NSuS^*" using rtrancl_trans[where ?r = ?NSuS] by blast
+  also have "\<dots> \<subseteq> S O ?NSuS^*" by regexp
   also have "\<dots> \<subseteq> S O (?NSS \<union> NS^*)"
     using compatible_rtrancl_split[where S = S and NS = NS] compat by blast
-  also have "\<dots> \<subseteq> ?NSS" using right_comp_S[where ?NS = NS and ?S = S] by blast
+  also have "\<dots> \<subseteq> ?NSS" by regexp
   finally have two: "?midS \<subseteq> ?NSS" . 
-
   from one two show ?thesis by auto 
 qed
 
@@ -1928,8 +2014,7 @@ proof-
     with  `(x, z) \<in> B^*` `(x, y) \<notin> B^*` have "(z, y) \<notin> B^*" by auto
     with Suc `(z, y) \<in> A ^^ i` have "(z, y) \<in> A^* O (A - B) O A^*" by auto
     with xz have xy:"(x, y) \<in> A O A\<^sup>* O (A - B) O A\<^sup>*" by auto
-    have "A O A\<^sup>* \<subseteq> A^*" by auto
-    hence "A O A\<^sup>* O (A - B) O A\<^sup>* \<subseteq> A\<^sup>* O (A - B) O A\<^sup>*" by auto
+    have "A O A\<^sup>* O (A - B) O A\<^sup>* \<subseteq> A\<^sup>* O (A - B) O A\<^sup>*" by regexp
     from this xy show "(x, y) \<in> A\<^sup>* O (A - B) O A\<^sup>*" using subsetD[where ?A="A O A\<^sup>* O (A - B) O A\<^sup>*"] by auto
   qed
  qed
@@ -1937,6 +2022,120 @@ qed
 
 lemma SN_empty[simp]: "SN {}" by auto
 
+
+lemma SN_elt_weakening:
+  assumes "SN_elt R1 a"
+  shows "SN_elt (R1 \<inter> R2) a"
+proof-
+{
+  assume "\<exists>S. S 0 = a \<and> (\<forall>i. (S i, S (Suc i)) \<in> R1 \<inter> R2)"
+  then obtain S where
+    S0: "S 0 = a" and
+    SN: "\<forall>i. (S i, S (Suc i)) \<in> (R1 \<inter> R2)"
+  by auto
+  from SN have SN': "\<forall>i. (S i, S (Suc i)) \<in> R1" by simp
+  with S0 and assms have "False" by auto
+}
+thus ?thesis by auto
+qed
+
+lemma SN_weakening:
+  assumes "SN R1"
+  shows "SN (R1 \<inter> R2)"
+using SN_elt_weakening and assms
+unfolding SN_def by metis
+
+lemma SN_elt_trancl_is_SN_elt: "SN_elt (r^+) = SN_elt r"
+proof (intro ext)
+  have r: "r \<subseteq> r^+" by auto
+  fix t
+  show "SN_elt (r^+) t = SN_elt r t"
+    using SN_elt_imp_SN_elt_trancl[of r t]
+    using SN_elt_subset[OF _ r, of t] by auto
+qed
+
+(* an explicit version of infinite reduction *)
+definition ideriv :: "'a ars \<Rightarrow> 'a ars \<Rightarrow> (nat \<Rightarrow> 'a) \<Rightarrow> bool"
+where "ideriv R S as \<equiv> (\<forall> i. (as i, as (Suc i)) \<in> R \<union> S) \<and> (INFM i. (as i,as (Suc i)) \<in> R)"
+
+lemma ideriv_mono: "R \<subseteq> R' \<Longrightarrow> S \<subseteq> S' \<Longrightarrow> ideriv R S as \<Longrightarrow> ideriv R' S' as"
+  unfolding ideriv_def INFM_nat by blast
+
+
+fun
+  shift :: "'a iseq \<Rightarrow> nat \<Rightarrow> 'a iseq"
+where
+  "shift f j = (\<lambda> i. f (i+j))"
+
+lemma ideriv_split: assumes ideriv: "ideriv R S as"
+  and nideriv: "\<not> ideriv (D \<inter> (R \<union> S)) (R \<union> S - D) as"
+  shows "\<exists> i. ideriv (R - D) (S - D) (shift as i)"
+proof -
+  have RS: "R - D \<union> (S - D) = R \<union> S - D" by auto
+  from ideriv[unfolded ideriv_def]
+  have as: "\<And> i. (as i, as (Suc i)) \<in> R \<union> S"
+    and inf: "INFM i. (as i, as (Suc i)) \<in> R" by auto
+  show ?thesis
+  proof (cases "INFM i. (as i, as (Suc i)) \<in> D \<inter> (R \<union> S)")
+    case True
+    have "ideriv (D \<inter> (R \<union> S)) (R \<union> S - D) as"
+      unfolding ideriv_def
+      using as True  by auto
+    with nideriv show ?thesis ..
+  next
+    case False
+    from False[unfolded INFM_nat]
+    obtain i where Dn: "\<And> j. i < j \<Longrightarrow> (as j, as (Suc j)) \<notin> D \<inter> (R \<union> S)"
+      by auto
+    from Dn as have as: "\<And> j. i < j \<Longrightarrow> (as j, as (Suc j)) \<in> R \<union> S - D" by auto
+    show ?thesis
+    proof (rule exI[of _ "Suc i"], unfold ideriv_def RS, insert as, intro conjI, simp, unfold INFM_nat, intro allI)
+      fix m
+      from inf[unfolded INFM_nat] obtain j where j: "j > Suc i + m" and R: "(as j, as (Suc j)) \<in> R" by auto
+      with as[of j] have RD: "(as j, as (Suc j)) \<in> R - D" by auto      
+      show "\<exists> j > m. (shift as (Suc i) j, shift as (Suc i) (Suc j)) \<in> R - D"
+        by (rule exI[of _ "j - Suc i"], insert j RD, auto)
+    qed
+  qed
+qed
+
+lemma ideriv_SN: assumes SN: "SN S"
+  and compat: "NS O S \<subseteq> S"
+  and R: "R \<subseteq> NS \<union> S"
+  shows "\<not> ideriv (S \<inter> R) (R - S) as"
+proof
+  assume "ideriv (S \<inter> R) (R - S) as"
+  with R have steps: "\<forall> i. (as i, as (Suc i)) \<in> NS \<union> S" and inf: "INFM i. (as i, as (Suc i)) \<in> S \<inter> R" unfolding ideriv_def by auto
+  from non_strict_ending[OF steps compat] SN
+  obtain i where i: "\<And> j. j \<ge> i \<Longrightarrow> (as j, as (Suc j)) \<in> NS - S" by auto
+  from inf[unfolded INFM_nat] obtain j where "j > i" and "(as j, as (Suc j)) \<in> S" by auto
+  with i[of j] show False by auto
+qed
+
+lemma Infm_shift: "(INFM i. P (shift f n i)) = (INFM i. P (f i))" (is "?S = ?O")
+proof 
+  assume ?S
+  show ?O
+    unfolding INFM_nat_le 
+  proof
+    fix m
+    from `?S`[unfolded INFM_nat_le]
+    obtain k where k: "k \<ge> m" and p: "P (shift f n k)" by auto
+    show "\<exists> k \<ge> m. P (f k)"
+      by (rule exI[of _ "k + n"], insert k p, auto)
+  qed
+next
+  assume ?O
+  show ?S
+    unfolding INFM_nat_le 
+  proof
+    fix m
+    from `?O`[unfolded INFM_nat_le]
+    obtain k where k: "k \<ge> m + n" and p: "P (f k)" by auto
+    show "\<exists> k \<ge> m. P (shift f n k)"
+      by (rule exI[of _ "k - n"], insert k p, auto)
+  qed
+qed
 
 subsection {* Relative Rewriting *}
 
@@ -1956,7 +2155,7 @@ fun
   rel_SN_alt :: "'a rel_ars \<Rightarrow> bool"
 where
   "rel_SN_alt (R, S) = (\<forall>(f::nat \<Rightarrow> 'a).
-    (\<forall>i. (f i, f (Suc i)) \<in> R \<union> S) \<longrightarrow> (\<exists>i. \<forall>j \<ge> i. (f j, f (Suc j)) \<notin> R))"
+    (\<forall>i. (f i, f (Suc i)) \<in> R \<union> S) \<longrightarrow> \<not> (INFM j. (f j, f (Suc j)) \<in> R))"
 
 lemma rel_SN_to_rel_SN_alt: "rel_SN (R, S) \<Longrightarrow> rel_SN_alt (R, S)"
 proof (unfold rel_SN_def)
@@ -1966,7 +2165,7 @@ proof (unfold rel_SN_def)
     fix f
     assume steps: "\<forall> i. (f i, f (Suc i)) \<in> R \<union> S"
     obtain r where  r: "\<And> j. r j \<equiv>  (f j, f (Suc j)) \<in> R" by auto
-    show "\<exists> i. \<forall> j \<ge> i. (f j, f (Suc j)) \<notin> R"
+    show "\<not> (INFM j. (f j, f (Suc j)) \<in> R)"
     proof (rule ccontr)
       assume "\<not> ?thesis"
       hence ih: "infinite_hits r" unfolding infinite_hits_def r by blast
@@ -2040,14 +2239,6 @@ next
     qed
   qed
 qed
-
-
-fun choice :: "(nat \<Rightarrow> 'a list) \<Rightarrow> nat \<Rightarrow> (nat \<times> nat)"
-where "choice f 0 = (0,0)"
-  |   "choice f (Suc n) = (let (i,j) = choice f n in 
-           if Suc j < length (f i) 
-               then (i,Suc j)
-               else (Suc i, 0))"
         
 lemma rel_SN_alt_to_rel_SN : "rel_SN_alt (R,S) \<Longrightarrow> rel_SN (R,S)"
 proof (unfold rel_SN_def)
@@ -2079,9 +2270,10 @@ proof (unfold rel_SN_def)
     from choice[OF this] obtain l where steps: "\<And> i. ?prop i (l i)" by auto
     let ?p = "\<lambda> i. ?prop i (l i)"
     from steps have steps: "\<And> i. ?p i" by blast
-    let ?l = "\<lambda> i. a i # l i"
-    let ?g = "\<lambda> i. choice (\<lambda> j. ?l j) i"
-    obtain g where g: "\<And> i. g i = (let (ii,jj) = ?g i in ?l ii ! jj)" by auto
+    let ?l = "\<lambda> i. a i # l i"    
+    let ?l' = "\<lambda> i. length (?l i)"
+    let ?g = "\<lambda> i. inf_concat_simple ?l' i"
+    obtain g where g: "\<And> i. g i = (let (ii,jj) = ?g i in ?l ii ! jj)" by auto    
     have len: "\<And> i j n. ?g n = (i,j) \<Longrightarrow> j < length (?l i)"
     proof -
       fix i j n
@@ -2125,21 +2317,15 @@ proof (unfold rel_SN_def)
         from gn gsn show ?thesis using steps[of i] steps[of "Suc i"] by auto
       qed
     qed
-    have infR:  "\<forall> n. \<exists> j \<ge> n. (g j, g (Suc j)) \<in> R" 
+    have infR:  "INFM j. (g j, g (Suc j)) \<in> R" unfolding INFM_nat_le
     proof
       fix n
       obtain i j where n: "?g n = (i,j)" by (cases "?g n", auto)
-      from len[OF n] have j: "j \<le> length (?l i) - 1" by simp
-      let ?k = "length (?l i) - 1 - j"
+      from len[OF n] have j: "j < ?l' i" .
+      let ?k = "?l' i - 1 - j"
       obtain k where k: "k = j + ?k" by auto
-      from j k have k2: "k = length (?l i) - 1" and k3: "j + ?k < length (?l i)" by auto
-      {
-        fix n i j k l
-        assume n: "choice l n = (i,j)" and "j + k < length (l i)"
-        hence "choice l (n + k) = (i, j + k)"
-          by (induct k arbitrary: j, simp, auto)
-      }
-      from this[OF n, of ?k, OF k3]
+      from j k have k2: "k = ?l' i - 1" and k3: "j + ?k < ?l' i" by auto
+      from inf_concat_simple_add[OF n, of ?k, OF k3] 
       have gnk: "?g (n + ?k) = (i, k)" by (simp only: k)
       hence "g (n + ?k) = ?l i ! k" unfolding g by auto
       hence gnk2: "g (n + ?k) = last (?l i)" using last_conv_nth[of "?l i"] k2 by auto
@@ -2150,11 +2336,10 @@ proof (unfold rel_SN_def)
       show "\<exists> j \<ge> n. (g j, g (Suc j)) \<in> R" 
         by (rule exI[of _ "n + ?k"], auto simp: main[simplified])
     qed      
-    from SN[simplified] gsteps infR show False by blast 
+    from SN[unfolded rel_SN_alt.simps] gsteps infR show False by blast 
   qed
 qed
 
-hide_const choice
 
 lemma rel_SN_conv : "rel_SN = rel_SN_alt"
   by (intro ext, clarify, intro iffI, rule rel_SN_to_rel_SN_alt, simp, rule rel_SN_alt_to_rel_SN, simp)
@@ -2276,6 +2461,541 @@ lemma rel_step_Id: "rel_step (R,S \<union> Id) = rel_step (R,S)"
 lemma rel_SN_Id:
   shows "rel_SN (R,S \<union> Id) = rel_SN (R,S)"
 unfolding rel_SN_def by (simp only: rel_step_Id)
+
+
+lemma rel_step_rtrancl: "rel_step (R,S^*) = rel_step (R,S)"
+  unfolding rel_step.simps rtrancl_idemp by simp
+
+lemma rel_SN_empty[simp]: "rel_SN (R,{}) = SN R"
+  unfolding rel_SN_def rel_step.simps by auto
+
+lemma rel_SN_ideriv: "rel_SN (R,S) = (\<not> (\<exists> as. ideriv R S as))" (is "?L = ?R")
+proof
+  assume ?L
+  show ?R
+  proof
+    assume "\<exists> as. ideriv R S as"
+    then obtain as where id: "ideriv R S as" by auto
+    note id = id[unfolded ideriv_def]
+    from `?L`[unfolded rel_SN_conv rel_SN_alt.simps, THEN spec[of _ as]]
+      id obtain i where i: "\<And> j. j \<ge> i \<Longrightarrow> (as j, as (Suc j)) \<notin> R" by auto
+    with id[unfolded INFM_nat, THEN conjunct2, THEN spec[of _ "Suc i"]] show False by auto
+  qed
+next
+  assume ?R
+  show ?L
+    unfolding rel_SN_conv rel_SN_alt.simps 
+  proof(intro allI impI)
+    fix as
+    assume "\<forall> i. (as i, as (Suc i)) \<in> R \<union> S"
+    with `?R`[unfolded ideriv_def] have "\<not> (INFM i. (as i, as (Suc i)) \<in> R)" by auto
+    from this[unfolded INFM_nat] obtain i where i: "\<And> j. i < j \<Longrightarrow> (as j, as (Suc j)) \<notin> R" by auto
+    show "\<not> (INFM j. (as j, as (Suc j)) \<in> R)" unfolding INFM_nat using i by blast
+  qed
+qed
+
+
+lemma rel_SN_map: fixes R Rw R' Rw' :: "'a ars" 
+  defines A: "A \<equiv> R' \<union> Rw'"
+  assumes SN: "rel_SN (R',Rw')" 
+  and R: "\<And> s t. (s,t) \<in> R \<Longrightarrow> (f s, f t) \<in> A^* O R' O A^*"
+  and Rw: "\<And> s t. (s,t) \<in> Rw \<Longrightarrow> (f s, f t) \<in> A^*"
+  shows "rel_SN (R,Rw)" 
+  unfolding rel_SN_def
+proof
+  fix g
+  assume steps: "\<forall> i. (g i, g (Suc i)) \<in> rel_step (R, Rw)"
+  let ?f = "\<lambda>i. (f (g i))"
+  obtain h where h: "h = ?f" by auto
+  {
+    fix i
+    let ?m = "\<lambda> (x,y). (f x, f y)"
+    {
+      fix s t
+      assume "(s,t) \<in> Rw^*"
+      hence "?m (s,t) \<in> A^*"
+      proof (induct)
+        case base show ?case by simp
+      next
+        case (step t u)
+        from Rw[OF step(2)] step(3)
+        show ?case by auto
+      qed
+    } note Rw = this
+    from steps have "(g i, g (Suc i)) \<in> rel_step (R,Rw)" ..
+    from this[unfolded rel_step.simps]
+    obtain s t where gs: "(g i,s) \<in> Rw^*" and st: "(s,t) \<in> R" and tg: "(t, g (Suc i)) \<in> Rw^*" by auto
+    from Rw[OF gs] R[OF st] Rw[OF tg]
+    have step: "(?f i, ?f (Suc i)) \<in> A^* O (A^* O R' O A^*) O A^*"
+      by auto
+    have "(?f i, ?f (Suc i)) \<in> A^* O R' O A^*"
+      by (rule set_mp[OF _ step], regexp)
+    hence "(h i, h (Suc i)) \<in> (rel_step (R',Rw'))^+"
+      unfolding A h rel_step_trancl_conv .
+  }
+  hence "\<not> SN ((rel_step (R',Rw'))^+)" by auto
+  with SN_imp_SN_trancl[OF SN[unfolded rel_SN_def]]
+  show False by simp
+qed
+
+datatype rel_SN_ext_type = top_s | top_ns | normal_s | normal_ns
+
+fun rel_SN_ext_step :: "'a ars \<Rightarrow> 'a ars \<Rightarrow> 'a ars \<Rightarrow> 'a ars \<Rightarrow> rel_SN_ext_type \<Rightarrow> 'a ars"
+  where "rel_SN_ext_step P Pw R Rw top_s = P"
+      | "rel_SN_ext_step P Pw R Rw top_ns = Pw"
+      | "rel_SN_ext_step P Pw R Rw normal_s = R"
+      | "rel_SN_ext_step P Pw R Rw normal_ns = Rw"
+
+(* relative termination with four relations as required in DP-framework *)
+definition rel_SN_ext :: "'a ars \<Rightarrow> 'a ars \<Rightarrow> 'a ars \<Rightarrow> 'a ars \<Rightarrow> ('a \<Rightarrow> bool) \<Rightarrow> bool"
+  where "rel_SN_ext P Pw R Rw M \<equiv> (\<not> (\<exists> f t. 
+       (\<forall> i. (f i, f (Suc i)) \<in> rel_SN_ext_step P Pw R Rw (t i))
+     \<and> (\<forall> i. M (f i))
+     \<and> (INFM i. t i \<in> {top_s,top_ns})
+     \<and> (INFM i. t i \<in> {top_s,normal_s})))"
+
+lemma rel_SN_ext_trans: fixes P Pw R Rw :: "'a ars" and M :: "'a \<Rightarrow> bool"
+  defines M': "M' \<equiv> {(s,t). M t}"
+  defines A: "A \<equiv> (P \<union> Pw \<union> R \<union> Rw) \<inter> M'"
+  assumes "rel_SN_ext P Pw R Rw M" 
+  shows "rel_SN_ext (A^* O (P \<inter> M') O A^*) (A^* O ((P \<union> Pw) \<inter> M') O A^*) (A^* O ((P \<union> R) \<inter> M') O A^*) (A^*) M" (is "rel_SN_ext ?P ?Pw ?R ?Rw M")
+proof (rule ccontr)
+  let ?relt = "rel_SN_ext_step ?P ?Pw ?R ?Rw"
+  let ?rel = "rel_SN_ext_step P Pw R Rw" 
+  assume "\<not> ?thesis"
+  from this[unfolded rel_SN_ext_def]
+  obtain f ty
+    where steps: "\<And> i. (f i, f (Suc i)) \<in> ?relt (ty i)" 
+    and min: "\<And> i. M (f i)"
+    and inf1: "INFM i. ty i \<in> {top_s, top_ns}"
+    and inf2: "INFM i. ty i \<in> {top_s, normal_s}"
+    by auto
+  let ?Un = "\<lambda> tt. \<Union> ?rel ` tt"
+  let ?UnM = "\<lambda> tt. (\<Union> ?rel ` tt) \<inter> M'"
+  let ?A = "?UnM {top_s,top_ns,normal_s,normal_ns}"
+  let ?P' = "?UnM {top_s}"
+  let ?Pw' = "?UnM {top_s,top_ns}"
+  let ?R' = "?UnM {top_s,normal_s}"
+  let ?Rw' = "?UnM {top_s,top_ns,normal_s,normal_ns}"
+  have A: "A = ?A" unfolding A by auto
+  have P: "(P \<inter> M') = ?P'" by auto
+  have Pw: "(P \<union> Pw) \<inter> M' = ?Pw'" by auto
+  have R: "(P \<union> R) \<inter> M' = ?R'" by auto
+  have Rw: "A = ?Rw'" unfolding A ..
+  {
+    fix s t tt
+    assume m: "M s" and st: "(s,t) \<in> ?UnM tt"
+    hence "\<exists> typ \<in> tt. (s,t) \<in> ?rel typ \<and> M s \<and> M t" unfolding M' by auto
+  } note one_step = this
+  let ?seq = "\<lambda> s t g n ty. s = g 0 \<and> t = g n \<and> (\<forall> i < n. (g i, g (Suc i)) \<in> ?rel (ty i)) \<and> (\<forall> i \<le> n. M (g i))"
+  {
+    fix s t
+    assume m: "M s" and st: "(s,t) \<in> A^*"
+    from st[unfolded rtrancl_fun_conv]
+    obtain g n where g0: "g 0 = s" and gn: "g n = t" and steps: "\<And> i. i < n \<Longrightarrow> (g i, g (Suc i)) \<in> ?A" unfolding A by auto
+    {
+      fix i
+      assume "i \<le> n"
+      have "M (g i)"
+      proof (cases i)
+        case 0
+        show ?thesis unfolding 0 g0 by (rule m)
+      next
+        case (Suc j)
+        with `i \<le> n` have "j < n" by auto
+        from steps[OF this] show ?thesis unfolding Suc M' by auto
+      qed
+    } note min = this
+    {
+      fix i
+      assume i: "i < n" hence i': "i \<le> n" by auto
+      from i' one_step[OF min steps[OF i]]
+      have "\<exists> ty. (g i, g (Suc i)) \<in> ?rel ty" by blast
+    }
+    hence "\<forall> i. (\<exists> ty. i < n \<longrightarrow> (g i, g (Suc i)) \<in> ?rel ty)" by auto
+    from choice[OF this]
+    obtain tt where steps: "\<And> i. i < n \<Longrightarrow> (g i, g (Suc i)) \<in> ?rel (tt i)" by auto
+    from g0 gn steps min
+    have "?seq s t g n tt" by auto
+    hence "\<exists> g n tt. ?seq s t g n tt" by blast
+  } note A_steps = this
+  let ?seqtt = "\<lambda> s t tt g n ty. s = g 0 \<and> t = g n \<and> n > 0 \<and> (\<forall> i<n. (g i, g (Suc i)) \<in> ?rel (ty i)) \<and> (\<forall> i \<le> n. M (g i)) \<and> (\<exists> i < n. ty i \<in> tt)"
+  {
+    fix s t tt
+    assume m: "M s" and st: "(s,t) \<in> A^* O ?UnM tt O A^*"
+    then obtain u v where su: "(s,u) \<in> A^*" and uv: "(u,v) \<in> ?UnM tt" and vt: "(v,t) \<in> A^*"
+      by auto
+    from A_steps[OF m su] obtain g1 n1 ty1 where seq1: "?seq s u g1 n1 ty1" by auto
+    from uv have "M v" unfolding M' by auto
+    from A_steps[OF this vt] obtain g2 n2 ty2 where seq2: "?seq v t g2 n2 ty2" by auto
+    from seq1 have "M u" by auto
+    from one_step[OF this uv] obtain ty where ty: "ty \<in> tt" and uv: "(u,v) \<in> ?rel ty" by auto
+    let ?g = "\<lambda> i. if i \<le> n1 then g1 i else g2 (i - (Suc n1))"
+    let ?ty = "\<lambda> i. if i < n1 then ty1 i else if i = n1 then ty else ty2 (i - (Suc n1))"
+    let ?n = "Suc (n1 + n2)"
+    have ex: "\<exists> i < ?n. ?ty i \<in> tt"
+      by (rule exI[of _ n1], simp add: ty)
+    have steps: "\<forall> i < ?n. (?g i, ?g (Suc i)) \<in> ?rel (?ty i)"
+    proof (intro allI impI)
+      fix i
+      assume "i < ?n"
+      show "(?g i, ?g (Suc i)) \<in> ?rel (?ty i)"
+      proof (cases "i \<le> n1")
+        case True
+        with seq1 seq2 uv show ?thesis by auto
+      next
+        case False
+        hence "i = Suc n1 + (i - Suc n1)" by auto
+        then obtain k where i: "i = Suc n1 + k" by auto
+        with `i < ?n` have "k < n2" by auto
+        thus ?thesis using seq2 unfolding i by auto
+      qed
+    qed
+    from steps seq1 seq2 ex 
+    have seq: "?seqtt s t tt ?g ?n ?ty" by auto
+    have "\<exists> g n ty. ?seqtt s t tt g n ty" 
+      by (intro exI, rule seq)
+  } note A_tt_A = this
+  let ?tycon = "\<lambda> ty1 ty2 tt ty' n. ty1 = ty2 \<longrightarrow> (\<exists>i < n. ty' i \<in> tt)"
+  let ?seqt = "\<lambda> i ty g n ty'. f i = g 0 \<and> f (Suc i) = g n \<and> (\<forall> j < n. (g j, g (Suc j)) \<in> ?rel (ty' j)) \<and> (\<forall> j \<le> n. M (g j)) 
+                \<and> (?tycon (ty i) top_s {top_s} ty' n)
+                \<and> (?tycon (ty i) top_ns {top_s,top_ns} ty' n)
+                \<and> (?tycon (ty i) normal_s {top_s,normal_s} ty' n)"
+  {
+    fix i
+    have "\<exists> g n ty'. ?seqt i ty g n ty'"
+    proof (cases "ty i")
+      case top_s
+      from steps[of i, unfolded top_s] 
+      have "(f i, f (Suc i)) \<in> ?P" by auto
+      from A_tt_A[OF min this[unfolded P]]
+      show ?thesis unfolding top_s by auto
+    next
+      case top_ns
+      from steps[of i, unfolded top_ns] 
+      have "(f i, f (Suc i)) \<in> ?Pw" by auto
+      from A_tt_A[OF min this[unfolded Pw]]
+      show ?thesis unfolding top_ns by auto
+    next
+      case normal_s
+      from steps[of i, unfolded normal_s] 
+      have "(f i, f (Suc i)) \<in> ?R" by auto
+      from A_tt_A[OF min this[unfolded R]]
+      show ?thesis unfolding normal_s by auto
+    next
+      case normal_ns
+      from steps[of i, unfolded normal_ns] 
+      have "(f i, f (Suc i)) \<in> ?Rw" by auto
+      from A_steps[OF min this]
+      show ?thesis unfolding normal_ns by auto
+    qed
+  }
+  hence "\<forall> i. \<exists> g n ty'. ?seqt i ty g n ty'" by auto
+  from choice[OF this] obtain g where "\<forall> i. \<exists> n ty'. ?seqt i ty (g i) n ty'" by auto
+  from choice[OF this] obtain n where "\<forall> i. \<exists> ty'. ?seqt i ty (g i) (n i) ty'" by auto
+  from choice[OF this] obtain ty' where "\<forall> i. ?seqt i ty (g i) (n i) (ty' i)" by auto
+  hence partial: "\<And> i. ?seqt i ty (g i) (n i) (ty' i)" ..
+  (* it remains to concatenate all these finite sequences to an infinite one *)
+  let ?ind = "inf_concat n"
+  let ?g = "\<lambda> k. (\<lambda> (i,j). g i j) (?ind k)"
+  let ?ty = "\<lambda> k. (\<lambda> (i,j). ty' i j) (?ind k)"
+  have inf: "INFM i. 0 < n i"
+    unfolding INFM_nat_le
+  proof (intro allI)
+    fix m
+    from inf1[unfolded INFM_nat_le]
+    obtain k where k: "k \<ge> m" and ty: "ty k \<in> {top_s, top_ns}" by auto
+    show "\<exists> k \<ge> m. 0 < n k"
+    proof (intro exI conjI, rule k)
+      from partial[of k] ty show "0 < n k" by (cases "n k", auto)
+    qed
+  qed
+  note bounds = inf_concat_bounds[OF inf]
+  note inf_Suc = inf_concat_Suc[OF inf]
+  note inf_mono = inf_concat_mono[OF inf]
+  have "\<not> rel_SN_ext P Pw R Rw M"
+    unfolding rel_SN_ext_def simp_thms
+  proof (rule exI[of _ ?g], rule exI[of _ ?ty], intro conjI allI)
+    fix k
+    obtain i j where ik: "?ind k = (i,j)" by force
+    from bounds[OF this] have j: "j < n i" by auto
+    show "M (?g k)" unfolding ik using partial[of i] j by auto
+  next
+    fix k
+    obtain i j where ik: "?ind k = (i,j)" by force
+    from bounds[OF this] have j: "j < n i" by auto
+    from partial[of i] j have step: "(g i j, g i (Suc j)) \<in> ?rel (ty' i j)" by auto
+    obtain i' j' where isk: "?ind (Suc k) = (i',j')" by force
+    have i'j': "g i' j' = g i (Suc j)"
+    proof (rule inf_Suc[OF _ ik isk])
+      fix i
+      from partial[of i]
+      have "g i (n i) = f (Suc i)" by simp
+      also have "... = g (Suc i) 0" using partial[of "Suc i"] by simp
+      finally show "g i (n i) = g (Suc i) 0" .
+    qed
+    show "(?g k, ?g (Suc k)) \<in> ?rel (?ty k)"
+      unfolding ik isk split i'j'
+      by (rule step)
+  next
+    show "INFM i. ?ty i \<in> {top_s, top_ns}"
+      unfolding INFM_nat_le
+    proof (intro allI)
+      fix k
+      obtain i j where ik: "?ind k = (i,j)" by force      
+      from inf1[unfolded INFM_nat] obtain i' where i': "i' > i" and ty: "ty i' \<in> {top_s, top_ns}" by auto
+      from partial[of i'] ty obtain j' where j': "j' < n i'" and ty': "ty' i' j' \<in> {top_s, top_ns}" by auto      
+      from inf_concat_surj[of _ n, OF j'] obtain k' where ik': "?ind k' = (i',j')" ..        
+      from inf_mono[OF ik ik' i'] have k: "k \<le> k'" by simp
+      show "\<exists> k' \<ge> k. ?ty k' \<in> {top_s, top_ns}"
+        by (intro exI conjI, rule k, unfold ik' split, rule ty')
+    qed
+  next
+    show "INFM i. ?ty i \<in> {top_s, normal_s}"
+      unfolding INFM_nat_le
+    proof (intro allI)
+      fix k
+      obtain i j where ik: "?ind k = (i,j)" by force      
+      from inf2[unfolded INFM_nat] obtain i' where i': "i' > i" and ty: "ty i' \<in> {top_s, normal_s}" by auto
+      from partial[of i'] ty obtain j' where j': "j' < n i'" and ty': "ty' i' j' \<in> {top_s, normal_s}" by auto
+      from inf_concat_surj[of _ n, OF j'] obtain k' where ik': "?ind k' = (i',j')" ..
+      from inf_mono[OF ik ik' i'] have k: "k \<le> k'" by simp
+      show "\<exists> k' \<ge> k. ?ty k' \<in> {top_s, normal_s}"
+        by (intro exI conjI, rule k, unfold ik' split, rule ty')
+    qed
+  qed
+  with assms show False by auto
+qed
+
+
+lemma rel_SN_ext_map: fixes P Pw R Rw P' Pw' R' Rw' :: "'a ars" and M M' :: "'a \<Rightarrow> bool"
+  defines Ms: "Ms \<equiv> {(s,t). M' t}"
+  defines A: "A \<equiv> (P' \<union> Pw' \<union> R' \<union> Rw') \<inter> Ms"
+  assumes SN: "rel_SN_ext P' Pw' R' Rw' M'" 
+  and P: "\<And> s t. M s \<Longrightarrow> M t \<Longrightarrow> (s,t) \<in> P \<Longrightarrow> (f s, f t) \<in> (A^* O (P' \<inter> Ms) O A^*) \<and> I t"
+  and Pw: "\<And> s t. M s \<Longrightarrow> M t \<Longrightarrow> (s,t) \<in> Pw \<Longrightarrow> (f s, f t) \<in> (A^* O ((P' \<union> Pw') \<inter> Ms) O A^*) \<and> I t"
+  and R: "\<And> s t. I s \<Longrightarrow> M s \<Longrightarrow> M t \<Longrightarrow> (s,t) \<in> R \<Longrightarrow> (f s, f t) \<in> (A^* O ((P' \<union> R') \<inter> Ms) O A^*) \<and> I t"
+  and Rw: "\<And> s t. I s \<Longrightarrow> M s \<Longrightarrow> M t \<Longrightarrow> (s,t) \<in> Rw \<Longrightarrow> (f s, f t) \<in> A^* \<and> I t"
+  shows "rel_SN_ext P Pw R Rw M" 
+proof -
+  note SN = rel_SN_ext_trans[OF SN]
+  let ?P = "(A^* O (P' \<inter> Ms) O A^*)"
+  let ?Pw = "(A^* O ((P' \<union> Pw') \<inter> Ms) O A^*)"
+  let ?R = "(A^* O ((P' \<union> R') \<inter> Ms) O A^*)"
+  let ?Rw = "A^*"
+  let ?relt = "rel_SN_ext_step ?P ?Pw ?R ?Rw"
+  let ?rel = "rel_SN_ext_step P Pw R Rw" 
+  show ?thesis 
+  proof (rule ccontr)
+    assume "\<not> ?thesis"
+    from this[unfolded rel_SN_ext_def]
+    obtain g ty
+      where steps: "\<And> i. (g i, g (Suc i)) \<in> ?rel (ty i)" 
+      and min: "\<And> i. M (g i)"
+      and inf1: "INFM i. ty i \<in> {top_s, top_ns}"
+      and inf2: "INFM i. ty i \<in> {top_s, normal_s}"
+      by auto
+    from inf1[unfolded INFM_nat] obtain k where k: "ty k \<in> {top_s, top_ns}" by auto
+    let ?k = "Suc k"
+    let ?i = "shift id ?k"
+    let ?f = "\<lambda> i. f (shift g ?k i)"
+    let ?ty = "shift ty ?k"
+    {
+      fix i
+      assume ty: "ty i \<in> {top_s,top_ns}"
+      note m = min[of i] 
+      note ms = min[of "Suc i"]
+      from P[OF m ms]
+        Pw[OF m ms]
+        steps[of i]
+        ty
+      have "(f (g i), f (g (Suc i))) \<in> ?relt (ty i) \<and> I (g (Suc i))"
+        by (cases "ty i", auto)
+    } note stepsP = this
+    {
+      fix i
+      assume I: "I (g i)"
+      note m = min[of i] 
+      note ms = min[of "Suc i"]
+      from P[OF m ms]
+        Pw[OF m ms]
+        R[OF I m ms]
+        Rw[OF I m ms]
+        steps[of i]
+      have "(f (g i), f (g (Suc i))) \<in> ?relt (ty i) \<and> I (g (Suc i))"
+        by (cases "ty i", auto)
+    } note stepsI = this
+    {
+      fix i
+      have "I (g (?i i))"
+      proof (induct i)
+        case 0
+        show ?case using stepsP[OF k] by simp
+      next
+        case (Suc i)
+        from stepsI[OF Suc] show ?case by simp
+      qed
+    } note I = this
+    have "\<not> rel_SN_ext ?P ?Pw ?R ?Rw M'"
+      unfolding rel_SN_ext_def simp_thms
+    proof (rule exI[of _ ?f], rule exI[of _ ?ty], intro allI conjI)
+      fix i
+      show "(?f i, ?f (Suc i)) \<in> ?relt (?ty i)"
+        using stepsI[OF I[of i]] by auto
+    next
+      show "INFM i. ?ty i \<in> {top_s, top_ns}"
+        unfolding Infm_shift[of "\<lambda>i. i \<in> {top_s,top_ns}" ty ?k]
+        by (rule inf1)
+    next
+      show "INFM i. ?ty i \<in> {top_s, normal_s}"
+        unfolding Infm_shift[of "\<lambda>i. i \<in> {top_s,normal_s}" ty ?k]
+        by (rule inf2)
+    next
+      fix i
+      have A: "A \<subseteq> Ms" unfolding A by auto
+      from rtrancl_mono[OF this] have As: "A^* \<subseteq> Ms^*" by auto
+      have PM: "?P \<subseteq> Ms^* O Ms O Ms^*" using As by auto
+      have PwM: "?Pw \<subseteq> Ms^* O Ms O Ms^*" using As by auto
+      have RM: "?R \<subseteq> Ms^* O Ms O Ms^*" using As by auto
+      have RwM: "?Rw \<subseteq> Ms^*" using As by auto
+      from PM PwM RM have "?P \<union> ?Pw \<union> ?R \<subseteq> Ms^* O Ms O Ms^*" (is "?PPR \<subseteq> _") by auto
+      also have "... \<subseteq> Ms^+" by regexp
+      also have "... = Ms"
+      proof
+        have "Ms^+ \<subseteq> Ms^* O Ms" by regexp
+        also have "... \<subseteq> Ms" unfolding Ms by auto
+        finally show "Ms^+ \<subseteq> Ms" .
+      qed regexp
+      finally have PPR: "?PPR \<subseteq> Ms" .
+      show "M' (?f i)"
+      proof (induct i)
+        case 0
+        from stepsP[OF k] k
+        have "(f (g k), f (g (Suc k))) \<in> ?PPR" by (cases "ty k", auto)
+        with PPR show ?case unfolding Ms by simp blast
+      next
+        case (Suc i)
+        show ?case
+        proof (cases "?ty i = normal_ns")
+          case False
+          hence "?ty i \<in> {top_s,top_ns,normal_s}"
+            by (cases "?ty i", auto)
+          with stepsI[OF I[of i]] have "(?f i, ?f (Suc i)) \<in> ?PPR"
+            by auto
+          from set_mp[OF PPR this] have "(?f i, ?f (Suc i)) \<in> Ms" .
+          thus ?thesis unfolding Ms by auto
+        next
+          case True
+          with stepsI[OF I[of i]] have "(?f i, ?f (Suc i)) \<in> ?Rw" by auto
+          with RwM have mem: "(?f i, ?f (Suc i)) \<in> Ms^*" by auto
+          thus ?thesis
+          proof (cases)
+            case base
+            with Suc show ?thesis by simp
+          next
+            case step
+            thus ?thesis unfolding Ms by simp
+          qed
+        qed
+      qed
+    qed
+    with SN
+    show False unfolding A Ms by simp
+  qed
+qed
+
+(* and a version where it is assumed that f always preserves M and that R' and Rw' preserve M' *)
+lemma rel_SN_ext_map_min: fixes P Pw R Rw P' Pw' R' Rw' :: "'a ars" and M M' :: "'a \<Rightarrow> bool"
+  defines Ms: "Ms \<equiv> {(s,t). M' t}"
+  defines A: "A \<equiv> P' \<inter> Ms \<union> Pw' \<inter> Ms \<union> R' \<union> Rw'"
+  assumes SN: "rel_SN_ext P' Pw' R' Rw' M'" 
+  and M: "\<And> t. M t \<Longrightarrow> M' (f t)"
+  and M': "\<And> s t. M' s \<Longrightarrow> (s,t) \<in> R' \<union> Rw' \<Longrightarrow> M' t"
+  and P: "\<And> s t. M s \<Longrightarrow> M t \<Longrightarrow> M' (f s) \<Longrightarrow> M' (f t) \<Longrightarrow> (s,t) \<in> P \<Longrightarrow> (f s, f t) \<in> (A^* O (P' \<inter> Ms) O A^*) \<and> I t"
+  and Pw: "\<And> s t. M s \<Longrightarrow> M t \<Longrightarrow> M' (f s) \<Longrightarrow> M' (f t) \<Longrightarrow> (s,t) \<in> Pw \<Longrightarrow> (f s, f t) \<in> (A^* O (P' \<inter> Ms \<union> Pw' \<inter> Ms) O A^*) \<and> I t"
+  and R: "\<And> s t. I s \<Longrightarrow> M s \<Longrightarrow> M t \<Longrightarrow> M' (f s) \<Longrightarrow> M' (f t) \<Longrightarrow> (s,t) \<in> R \<Longrightarrow> (f s, f t) \<in> (A^* O (P' \<inter> Ms \<union> R') O A^*) \<and> I t"
+  and Rw: "\<And> s t. I s \<Longrightarrow> M s \<Longrightarrow> M t \<Longrightarrow> M' (f s) \<Longrightarrow> M' (f t) \<Longrightarrow> (s,t) \<in> Rw \<Longrightarrow> (f s, f t) \<in> A^* \<and> I t"
+  shows "rel_SN_ext P Pw R Rw M"  
+proof -
+  let ?Ms = "{(s,t). M' t}"
+  let ?A = "(P' \<union> Pw' \<union> R' \<union> Rw') \<inter> ?Ms"
+  {
+    fix s t
+    assume s: "M' s" and "(s,t) \<in> A" 
+    with M'[OF s, of t] have "(s,t) \<in> ?A \<and> M' t" unfolding Ms A by auto
+  } note Aone = this
+  {
+    fix s t
+    assume s: "M' s" and steps: "(s,t) \<in> A^*"
+    from steps have "(s,t) \<in> ?A^* \<and> M' t"
+    proof (induct)
+      case base from s show ?case by simp
+    next
+      case (step t u)
+      note one = Aone[OF step(3)[THEN conjunct2] step(2)] 
+      from step(3) one
+      have steps: "(s,u) \<in> ?A^* O ?A" by blast      
+      have "(s,u) \<in> ?A^*" 
+        by (rule set_mp[OF _ steps], regexp)
+      with one show ?case by simp
+    qed
+  } note Amany = this      
+  let ?P = "(A^* O (P' \<inter> Ms) O A^*)"
+  let ?Pw = "(A^* O (P' \<inter> Ms \<union> Pw' \<inter> Ms) O A^*)"
+  let ?R = "(A^* O (P' \<inter> Ms \<union> R') O A^*)"
+  let ?Rw = "A^*"
+  let ?P' = "(?A^* O (P' \<inter> ?Ms) O ?A^*)"
+  let ?Pw' = "(?A^* O ((P' \<union> Pw') \<inter> ?Ms) O ?A^*)"
+  let ?R' = "(?A^* O ((P' \<union> R') \<inter> ?Ms) O ?A^*)"
+  let ?Rw' = "?A^*"
+  show ?thesis 
+  proof (rule rel_SN_ext_map[OF SN])
+    fix s t
+    assume s: "M s" and t: "M t" and step: "(s,t) \<in> P"
+    from P[OF s t M[OF s] M[OF t] step]
+    have "(f s, f t) \<in> ?P" and I: "I t"  by auto
+    then obtain u v where su: "(f s, u) \<in> A^*" and uv: "(u,v) \<in> P' \<inter> Ms"
+      and vt: "(v,f t) \<in> A^*" by auto
+    from Amany[OF M[OF s] su] have su: "(f s, u) \<in> ?A^*" and u: "M' u" by auto
+    from uv have v: "M' v" unfolding Ms by auto
+    from Amany[OF v vt] have vt: "(v, f t) \<in> ?A^*" by auto
+    from su uv vt I 
+    show "(f s, f t) \<in> ?P' \<and> I t" unfolding Ms by auto
+  next
+    fix s t
+    assume s: "M s" and t: "M t" and step: "(s,t) \<in> Pw"
+    from Pw[OF s t M[OF s] M[OF t] step]
+    have "(f s, f t) \<in> ?Pw" and I: "I t"  by auto
+    then obtain u v where su: "(f s, u) \<in> A^*" and uv: "(u,v) \<in> P' \<inter> Ms \<union> Pw' \<inter> Ms"
+      and vt: "(v,f t) \<in> A^*" by auto
+    from Amany[OF M[OF s] su] have su: "(f s, u) \<in> ?A^*" and u: "M' u" by auto
+    from uv have uv: "(u,v) \<in> (P' \<union> Pw') \<inter> ?Ms" and v: "M' v" unfolding Ms 
+      by auto
+    from Amany[OF v vt] have vt: "(v, f t) \<in> ?A^*" by auto
+    from su uv vt I 
+    show "(f s, f t) \<in> ?Pw' \<and> I t"  by auto
+  next
+    fix s t
+    assume I: "I s" and s: "M s" and t: "M t" and step: "(s,t) \<in> R"
+    from R[OF I s t M[OF s] M[OF t] step]
+    have "(f s, f t) \<in> ?R" and I: "I t"  by auto
+    then obtain u v where su: "(f s, u) \<in> A^*" and uv: "(u,v) \<in> P' \<inter> Ms \<union> R'"
+      and vt: "(v,f t) \<in> A^*" by auto
+    from Amany[OF M[OF s] su] have su: "(f s, u) \<in> ?A^*" and u: "M' u" by auto
+    from uv M'[OF u, of v] have uv: "(u,v) \<in> (P' \<union> R') \<inter> ?Ms" and v: "M' v" unfolding Ms 
+      by auto
+    from Amany[OF v vt] have vt: "(v, f t) \<in> ?A^*" by auto
+    from su uv vt I 
+    show "(f s, f t) \<in> ?R' \<and> I t"  by auto
+  next
+    fix s t
+    assume I: "I s" and s: "M s" and t: "M t" and step: "(s,t) \<in> Rw"
+    from Rw[OF I s t M[OF s] M[OF t] step]
+    have steps: "(f s, f t) \<in> ?Rw" and I: "I t"  by auto
+    from Amany[OF M[OF s] steps] I
+    show "(f s, f t) \<in> ?Rw' \<and> I t"  by auto
+  qed
+qed
 
 
 end
